{
 "cells": [
  {
   "cell_type": "markdown",
   "metadata": {},
   "source": [
    "<h3 style=\"text-align: center;\"><strong>Variance</strong></h3>\n",
    "<h3 style=\"text-align: center;\"><strong>Covariance</strong></h3>\n",
    "<h3 style=\"text-align: center;\"><strong>Standard deviation</strong></h3>\n",
    "<h3 style=\"text-align: center;\"><strong>Correlation</strong></h3>\n",
    "\n",
    "<br><br>\n",
    "\n",
    "<p>Mean(average) is the \"center weight\" of the data</p>\n",
    "<p>Population mean: <span class=\"f\"> $\\mu = {\\sum_{i=1}^{n} x_{i} \\over n}$</span></p>\n",
    "<p>Sample mean: <span class=\"f\">$\\bar{x} = {\\sum_{i=1}^{n} x_{i} \\over n}$</span></p>\n",
    "<p>The sum of deviations of data values from the mean is zero: $\\sum _{ i=1 }^{ n }{ ({ x }_{ i }-mean) = 0 } $ </p>\n",
    "\n",
    "<hr>\n",
    "\n",
    "<p>Variance: measure of variability (spread around) the mean</p>\n",
    "<p>(not standardized - scale dependent)</p>\n",
    "<p>Population variance: <span class=\"f\">$\\sigma^2={\\sum_{i=1}^{n} (x_{i}-\\mu)^2 \\over n}$</span></p>\n",
    "<p>Sample variance: <span class=\"f\">$S^2={\\sum_{i=1}^{n} (x_{i}-\\bar{x})^2 \\over n-1}$</span></p>\n",
    "\n",
    "<hr>\n",
    "\n",
    "<p>Standard deviation: measure of variability (spread around) the mean</p>\n",
    "<p>(standardized - not scale dependend - adimensional)</p>\n",
    "<p>Standard deviation for population: <span class=\"f\">$\\sigma = \\sqrt{\\sum_{i=1}^{n}{(x_i - \\mu)}^2 \\over n}$</span></p>\n",
    "<p>Standard deviation for a sample: <span class=\"f\">$S = \\sqrt{\\sum_{i=1}^{n}{(x_i - \\bar{x})}^2 \\over n - 1}$</span></p>\n",
    "\n",
    "<hr>\n",
    "\n",
    "<p>Covariance: measure of relationship between the variances(variability) of two variables</p>\n",
    "<p>(not standardized - scale dependent)</p>\n",
    "<p>Population covariance: <span class=\"f\">$cov(x,y)=\\frac { \\sum _{ i=1 }^{ n }{ ({ x }_{ i }-{ \\mu }_{ x } )({ y }_{ i }-{ \\mu }_{ y } ) }  }{ n } $</span></p>\n",
    "<p>Sample covariance: <span class=\"f\">$cov(x,y)=\\frac { \\sum _{ i=1 }^{ n }{ ({ x }_{ i }-\\overline { x } )({ y }_{ i }-\\overline { y } ) }  }{ n-1 } $</span></p>\n",
    "\n",
    "<hr>\n",
    "\n",
    "<p>Correlation(Pearson coefficient): measure of relationship between the variances(variability) of two variables</p>\n",
    "<p>(standardized - not scale dependend - adimensional)</p>\n",
    "\n",
    "<p>Population: <span class=\"f\">$ { r }_{ pop }=cor(x,y)=\\frac { cov(x,y) }{ { \\sigma  }_{ x }{ \\sigma  }_{ y } } =\\frac { \\frac { 1 }{ n } \\sum _{ i=1 }^{ n }{ ({ x }_{ i }-{ \\mu  }_{ x })({ y }_{ i }-{ \\mu  }_{ y }) }  }{ \\sqrt { \\frac { 1 }{ n } \\sum _{ i=1 }^{ n }{ { ({ x }_{ i }-{ \\mu  }_{ x }) }^{ 2 } }  } \\sqrt { \\frac { 1 }{ n } \\sum _{ i=1 }^{ n }{ { ({ y }_{ i }-{ \\mu  }_{ y }) }^{ 2 } }  }  } $</span></p>\n",
    "\n",
    "<p><span class=\"f\">$ { r }_{ pop }=\\frac { \\sum { ({ x }-{ \\mu  }_{ x })({ y }-{ \\mu  }_{ y }) }  }{ \\sqrt { \\sum { { ({ x }-{ \\mu  }_{ x }) }^{ 2 } }  } \\sqrt { \\sum { { ({ y }-{ \\mu  }_{ y }) }^{ 2 } }  }  } =\\frac { n\\sum { xy-\\sum { x\\sum { y }  }  }  }{ \\sqrt { n\\sum { { x }^{ 2 }-({ \\sum { x) }  }^{ 2 } }  } \\sqrt { n\\sum { { y }^{ 2 }-({ \\sum { y) }  }^{ 2 } }  }  } $</span></p>\n",
    "\n",
    "<p>Sample: <span class=\"f\">$ { r }_{ sample }=cor(x,y)=\\frac { cov(x,y) }{ { \\sigma  }_{ x }{ \\sigma  }_{ y } } =\\frac { \\frac { 1 }{ n-1 } \\sum _{ i=1 }^{ n }{ ({ x }_{ i }-\\overline { x } )({ y }_{ i }-\\overline { y } ) }  }{ \\sqrt { \\frac { 1 }{ n-1 } \\sum _{ i=1 }^{ n }{ { ({ x }_{ i }-\\overline { x } ) }^{ 2 } }  } \\sqrt { \\frac { 1 }{ n-1 } \\sum _{ i=1 }^{ n }{ { ({ y }_{ i }-\\overline { y } ) }^{ 2 } }  }  }   $</span></p>\n",
    "\n",
    "<p><span class=\"f\">$ { r }_{ sample }=\\frac { \\sum { ({ x }-\\overline { x } )({ y }-\\overline { y } ) }  }{ \\sqrt { \\sum { { ({ x }-{ \\overline { x }  }) }^{ 2 } }  } \\sqrt { \\sum { { ({ y }-{ \\overline { y }  }) }^{ 2 } }  }  } =\\frac { n\\sum { xy-\\sum { x\\sum { y }  }  }  }{ \\sqrt { n\\sum { { x }^{ 2 }-({ \\sum { x) }  }^{ 2 } }  } \\sqrt { n\\sum { { y }^{ 2 }-({ \\sum { y) }  }^{ 2 } }  }  }   $</span></p>\n",
    "\n",
    "<p>see proof1-below</p>\n",
    "\n",
    "<hr>\n",
    "\n",
    "<p>Slope of regression line</p>\n",
    "\n",
    "<p><span class=\"f\">$ m=r\\frac { { \\sigma  }_{ y } }{ { \\sigma  }_{ x } } =\\frac { \\frac { \\sum { xy }  }{ n } -{ \\mu  }_{ x }{ \\mu  }_{ y } }{ \\frac { \\sum { { x }^{ 2 } }  }{ n } -{ { (\\mu  }_{ x }) }^{ 2 } } =\\frac { { \\mu  }_{ xy }-{ \\mu  }_{ x }{ \\mu  }_{ y } }{ { \\mu  }_{ { x }^{ 2 } }-{ { (\\mu  }_{ x }) }^{ 2 } } $</span></p>\n",
    "\n",
    "<p><span class=\"f\">$ m=r\\frac { { S }_{ y } }{ { S }_{ x } } =\\frac { \\frac { \\sum { xy }  }{ n } -\\overline { x } \\cdot \\overline { y }  }{ \\frac { \\sum { { x }^{ 2 } }  }{ n } -{ (\\overline { x } ) }^{ 2 } } =\\frac { \\overline { xy } -\\overline { x } \\cdot \\overline { y }  }{ \\overline { { x }^{ 2 } } -{ (\\overline { x } ) }^{ 2 } }  $</span></p>\n",
    "\n",
    "<p>see proof2-below</p>\n",
    "\n",
    "<hr>\n",
    "<br>\n",
    "\n",
    "<p><u>Proof1</u></p>\n",
    "\n",
    "<p>$ { r }_{ sample }=cor(x,y)=\\frac { cov(x,y) }{ { \\sigma  }_{ x }{ \\sigma  }_{ y } } =\\frac { \\frac { 1 }{ n-1 } \\sum _{ i=1 }^{ n }{ ({ x }_{ i }-\\overline { x } )({ y }_{ i }-\\overline { y } ) }  }{ \\sqrt { \\frac { 1 }{ n-1 } \\sum _{ i=1 }^{ n }{ { ({ x }_{ i }-\\overline { x } ) }^{ 2 } }  } \\sqrt { \\frac { 1 }{ n-1 } \\sum _{ i=1 }^{ n }{ { ({ y }_{ i }-\\overline { y } ) }^{ 2 } }  }  } =\\frac { \\sum { ({ x }-\\overline { x } )({ y }-\\overline { y } ) }  }{ \\sqrt { \\sum { { ({ x }_{ i }-\\overline { x } ) }^{ 2 } }  } \\sqrt { \\sum { { ({ y }_{ i }-\\overline { y } ) }^{ 2 } }  }  }   $</p>\n",
    "\n",
    "\n",
    "<p>Having these relations:</p>\n",
    "\n",
    "<p>$ \\overline { x } =\\frac { \\sum { x }  }{ n } \\Rightarrow \\sum { x } =n\\overline { x } \\\\ \\overline { y } =\\frac { \\sum { y }  }{ n } \\Rightarrow \\sum { y } =n\\overline { y } \\\\ \\sum { (x-\\overline { x } )=0 } \\\\ \\sum { (y-\\overline { y } )=0 }   $</p>\n",
    "\n",
    "<p>Will follow:</p>\n",
    "\n",
    "<p>Nominator:</p>\n",
    "\n",
    "<p>$\\sum { (x-\\overline { x } )(y-\\overline { y } ) } =\\sum { \\left\\{ y(x-\\overline { x } )-\\overline { y } (x-\\overline { x } ) \\right\\}  } =\\\\ =\\sum { xy } -\\sum { \\overline { x }  } y-\\sum { \\overline { y } (x-\\overline { x } ) } =\\\\ =\\sum { xy } -\\overline { x } \\sum { y } -\\overline { y } \\sum { (x-\\overline { x } ) } =\\\\ =\\sum { xy } -\\overline { x } ny - \\overline { y } \\cdot 0=\\\\ =\\sum { xy } -n\\overline { x } \\overline { y } $</p>\n",
    "\n",
    "<p>Denominator:</p>\n",
    "\n",
    "<p>$\\sum { { (x-\\overline { x } ) }^{ 2 } } =\\sum { (x-\\overline { x } )(x-\\overline { x } )= } \\\\ =\\sum { x } (x-\\overline { x } )\\quad -\\quad \\overline { x } \\sum { (x-\\overline { x } ) } =\\\\ =\\sum { { x }^{ 2 } } -\\overline { x } \\sum { x } -\\quad \\overline { x } \\cdot 0=\\\\ =\\sum { { x }^{ 2 } } -\\quad \\overline { x } n\\overline { x } =\\sum { { x }^{ 2 } } -n{ \\overline { x }  }^{ 2 }$</p>\n",
    "\n",
    "<p>Similarly:</p>\n",
    "\n",
    "<p>$\\sum { { (y-\\overline { y } ) }^{ 2 } } =\\sum { { y }^{ 2 } } -n{ \\overline { y }  }^{ 2 }$</p>\n",
    "\n",
    "<p>So:</p>\n",
    "\n",
    "<p>$r=\\frac { \\sum { xy } -n\\overline { x } \\overline { y }  }{ \\sqrt { \\sum { { x }^{ 2 } } -n{ \\overline { x }  }^{ 2 } } \\sqrt { \\sum { { y }^{ 2 } } -n{ \\overline { y }  }^{ 2 } }  } =\\frac { \\sum { xy } -n\\frac { \\sum { x }  }{ n } \\frac { \\sum { y }  }{ n }  }{ \\sqrt { \\sum { { x }^{ 2 } } -n\\frac { { (\\sum { x) }  }^{ 2 } }{ { n }^{ 2 } }  } \\sqrt { \\sum { { y }^{ 2 } } -n\\frac { { (\\sum { y) }  }^{ 2 } }{ { n }^{ 2 } }  }  } =$</p>\n",
    "\n",
    "<p>$=\\frac { \\sum { xy } -\\frac { 1 }{ n } \\sum { x } \\sum { y }  }{ \\sqrt { \\sum { { x }^{ 2 } } -\\frac { { (\\sum { x) }  }^{ 2 } }{ { n } }  } \\sqrt { \\sum { { y }^{ 2 } } -\\frac { { (\\sum { y) }  }^{ 2 } }{ { n } }  }  } =$ (multiplying with n at nominator and denominator) </p>\n",
    "\n",
    "<p>$ =\\frac { n\\sum { xy-\\sum { x\\sum { y }  }  }  }{ \\sqrt { n\\sum { { x }^{ 2 }-({ \\sum { x) }  }^{ 2 } }  } \\sqrt { n\\sum { { y }^{ 2 }-({ \\sum { y) }  }^{ 2 } }  }  }   $</p>\n",
    "\n",
    "\n",
    "<p><u>Proof 2</u></p>\n",
    "\n",
    "<p>$ m=r\\frac { { S }_{ y } }{ { S }_{ x } } =\\frac { \\sum { ({ x }-\\overline { x } )({ y }-\\overline { y } ) }  }{ \\sqrt { \\sum { { ({ x }-{ \\overline { x }  }) }^{ 2 } }  } \\sqrt { \\sum { { ({ y }-{ \\overline { y }  }) }^{ 2 } }  }  } \\cdot \\frac { \\sqrt { \\sum { { ({ y }-{ \\overline { y }  }) }^{ 2 } }  }  }{ \\sqrt { \\sum { { ({ x }-{ \\overline { x }  }) }^{ 2 } }  }  } =\\\\ =\\frac { \\sum { ({ x }-\\overline { x } )({ y }-\\overline { y } ) }  }{ \\sum { { ({ x }-{ \\overline { x }  }) }^{ 2 } }  } =\\frac { \\sum { xy } -n\\overline { x } \\overline { y }  }{ \\sum { { x }^{ 2 }-n{ \\overline { x }  }^{ 2 } }  } =\\frac { \\frac { \\sum { xy }  }{ n } -\\overline { x } \\overline { y }  }{ \\frac { \\sum { { x }^{ 2 } }  }{ n } -{ \\overline { x }  }^{ 2 } } =\\frac { \\overline { xy } -\\overline { x } \\overline { y }  }{ \\overline { { x }^{ 2 } } -{ \\overline { x }  }^{ 2 } }  $</p>\n",
    "\n"
   ]
  },
  {
   "cell_type": "code",
   "execution_count": null,
   "metadata": {},
   "outputs": [],
   "source": []
  }
 ],
 "metadata": {
  "kernelspec": {
   "display_name": "Python 3",
   "language": "python",
   "name": "python3"
  },
  "language_info": {
   "codemirror_mode": {
    "name": "ipython",
    "version": 3
   },
   "file_extension": ".py",
   "mimetype": "text/x-python",
   "name": "python",
   "nbconvert_exporter": "python",
   "pygments_lexer": "ipython3",
   "version": "3.7.1"
  }
 },
 "nbformat": 4,
 "nbformat_minor": 2
}
